\documentclass[12pt]{article}

\usepackage[margin=1in]{geometry} 
\usepackage{amsmath,amsthm,amssymb}
\usepackage{lscape}

\begin{document}
	
\begin{equation}
M\mathbf{\ddot{x}} + \Lambda\mathbf{\dot{x}} + K\mathbf{x} = \mathbf{f}
\end{equation}
	
	
\begin{math}	
\begin{aligned}
\mathbf{x} &= 
\begin{bmatrix} 
	x_{f1} \\
	x_{f2} \\
	x_{f3} \\
	x_{a1} \\
	x_{a2} \\
	x_{a3} \\
\end{bmatrix} \\
\mathbf{f} &= 
\begin{bmatrix} 
	Fsin(\omega t) \\
	0 \\
	0 \\
	0 \\
	0 \\
	0 \\
\end{bmatrix} \\	
M &=
\begin{bmatrix} 
 m & 0 & 0 & 0 & 0 & 0 \\
 0 & m & 0 & 0 & 0 & 0 \\
 0 & 0 & m & 0 & 0 & 0 \\
 0 & 0 & 0 & m_{a1} & 0 & 0 \\
 0 & 0 & 0 & 0 & m_{a2} & 0 \\
 0 & 0 & 0 & 0 & 0 & m_{a3} \\
\end{bmatrix}  \\
\Lambda &= 
\begin{bmatrix} 
 \lambda_{f1} + \lambda_{f2} + \lambda_{a1} & -\lambda{f1} & 0 & -\lambda_{a1} & 0 & 0 \\
 -\lambda{f2} & \lambda{f2} + \lambda{f3} + \lambda{a2} & -\lambda{f3} & 0 & -\lambda{a2} & 0 \\
 0 & -\lambda{f2} & \lambda{f3} + \lambda{a3} & 0 & 0 & -\lambda{a3} \\
 -\lambda{f1} & 0 & 0 & \lambda{a1} & 0 & 0 \\
 0 & -\lambda{f2} & 0 & 0 & \lambda{a2} & 0 \\
 0 & 0 & -\lambda{f3} & 0 & 0 & \lambda{a3} \\
 \end{bmatrix} \\
K &= 
\begin{bmatrix} 
 k_{f1} + k_{f2} +  k_{a1} & -k_{f2} & 0 & -k_{a1} & 0 & 0 \\
 -k_{f2} & k_{f2} + k_{f3} + k_{a2} & -k{f3} & 0 & -k_{a2} & 0 \\
 0 & -k_{f2} & k_{f3} + k_{a2} & 0 & 0 & -k_{a3} \\
 -k_{f1} & 0 & 0 & k_{a1} & 0 & 0 \\
 0 & -k_{f2} & 0 & 0 & k_{a2} & 0 \\
 0 & 0 & -k_{f3} & 0 & 0 & k_{a3} \\
\end{bmatrix} \\
\end{aligned}
\end{math}


\end{document}          
