\begin{bmatrix} 
 m_{f1} & 0 & 0 & 0 & 0 & 0 \\
 0 & m_{f2} & 0 & 0 & 0 & 0 \\
 0 & 0 & m_{f3} & 0 & 0 & 0 \\
 0 & 0 & 0 & m_{a1} & 0 & 0 \\
 0 & 0 & 0 & 0 & m_{a2} & 0 \\
 0 & 0 & 0 & 0 & 0 & m_{a3} \\
\end{bmatrix} 
\mathbf{\ddot{x}} 
+ 
\begin{bmatrix} 
 \lambda_{f1} + \lambda_{f2} + \lambda_{a1} & -\lambda{f1} & 0 & -\lambda_{a1} & 0 & 0 \\
 -\lambda{f2} & \lambda{f2} + \lambda{f3} + \lambda{a2} & -\lambda{f3} & 0 & -\lambda{a2} & 0 \\
 0 & -\lambda{f2} & \lambda{f3} + \lambda{a3} & 0 & 0 & -\lambda{a3} \\
 -\lambda{f1} & 0 & 0 & \lambda{a1} & 0 & 0 \\
 0 & -\lambda{f2} & 0 & 0 & \lambda{a2} & 0 \\
 0 & 0 & -\lambda{f3} & 0 & 0 & \lambda{a3} \\
 \end{bmatrix} 
\mathbf{\dot{x}} 
+
\begin{bmatrix} \lambda_{f1} + \lambda_{f2} + \lambda_{a1} & -\lambda{f1} & 0 & -\lambda_{a1} & 0 & 0 \\
 -\lambda{f2} & \lambda{f2} + \lambda{f3} + \lambda{a2} & -\lambda{f3} & 0 & -\lambda{a2} & 0 \\
 0 & -\lambda{f2} & \lambda{f3} + \lambda{a3} & 0 & 0 & -\lambda{a3} \\
 -\lambda{f1} & 0 & 0 & \lambda{a1} & 0 & 0 \\
 0 & -\lambda{f2} & 0 & 0 & \lambda{a2} & 0 \\
 0 & 0 & -\lambda{f3} & 0 & 0 & \lambda{a3} \\
\end{bmatrix} 
\mathbf{\dot{x}}
+
\begin{bmatrix}
 
 k_{f1} + k_{f2} +  k_{a1} & -k_{f2} & 0 & -k_{a1} & 0 & 0 \\
 -k_{f2} & k_{f2} + k_{f3} + k_{a2} & -k{f3} & 0 & -k_{a2} & 0 \\
 0 & -k_{f2} & k_{f3} + k_{a2} & 0 & 0 & -k_{a3} \\
 -k_{f1} & 0 & 0 & k_{a1} & 0 & 0 \\
 0 & -k_{f2} & 0 & 0 & k_{a2} & 0 \\
 0 & 0 & -k_{f3} & 0 & 0 & k_{a3} \\

\end{bmatrix}
\mathbf{x}
=
\mathbf{f}
